

## Recap. Group algebra

1. group elements, operators/actions & vectors/objects

$$\mathbb{C}[G] = \left\{ \sum_g \alpha_g \cdot g \mid \alpha_g \in \mathbb{C} \right\}$$

$$\begin{cases} x+y = \sum_g (x(g) + y(g)) \cdot g \\ \alpha x = \sum_g (\alpha x(g)) \cdot g \\ x \cdot y = \sum_g x(g) y(g^{-1}k) \cdot k \end{cases}$$

$$L(h) \cdot x = L(h) \sum_g x(g) \cdot g = \sum_g x(g) (hg) = \sum_g x(h^{-1}g) g$$

$$\Rightarrow [L(h) \cdot x](g) = x(h^{-1}g)$$

$$x = \delta_g \Rightarrow h \cdot \delta_g = \delta_{hg}$$

2. Define class operators

$$C_i = \sum_{g \in G_i} g \in \text{End}_{\mathbb{C}}(\mathbb{C}[G])$$

then  $[C_i, g] = 0$  ( $\forall g \in G$ ), intertwiners

All  $\{C_i\}$  commute  $\Rightarrow$  can be simultaneously

diagonalized. we can represent them

within the center of  $\mathbb{C}[G]$ :  $\text{span}\{C_i\}$

$$\boxed{\hat{C}_i \cdot \hat{C}_j = \sum_k D_{ij}^k \hat{C}_k} \quad D_{ij} \text{ are the}$$

recall matrix rep:

$$\begin{aligned} g \cdot e_i &= \sum_j \mu_{ji}(g) e_j \\ \uparrow \quad \uparrow \\ \hat{C}_j \quad C_i &= \sum_k D(j)_k C_k \end{aligned}$$

what are the eigenvectors?

$$\hat{C}_j \vec{\phi}^{(\mu)} = \lambda_\mu \vec{\phi}^{(\mu)}$$

We have shown that assuming nondegeneracy

What if there is degeneracy? Find another  $C_i$  that splits the degeneracy.

$\Rightarrow$  We will see later that there is no degeneracy

if all  $\{C_i\}$  are diagonalized. (CSCD-I)

$$\hat{C}_j \vec{\phi}^\mu \vec{\phi}^\nu = (\lambda^\mu \vec{\phi}^\mu) \vec{\phi}^\nu = \phi^\mu (\lambda^\mu \vec{\phi}^\nu) = \lambda^\mu \delta_{\mu\nu} \vec{\phi}^\mu \vec{\phi}^\nu$$

$\{\vec{\phi}^\mu\}$  behave like projectors!

$$\hat{C}_i \vec{\phi} = \lambda_i \vec{\phi} \quad \text{then} \quad \vec{\phi} = \sum_{i=1}^r \alpha_i C_i$$

$$C_i \vec{\phi} = C_i \sum_j \alpha_j C_j = \sum_j \alpha_j C_i C_j = \sum_{j \neq i} \alpha_j D_{ij}^k C_k$$

$$\equiv \lambda_i \vec{\phi} = \lambda_i \sum_j \alpha_j C_j = \sum_k (\lambda_i \alpha_k) C_k$$

$$\Rightarrow \sum_j \alpha_j D_{ij}^k = \lambda_i \alpha_k$$

$$\vec{\phi}^2 = \sum_{ij} \alpha_i \alpha_j C_i C_j = \sum_{ij} \alpha_i \alpha_j D_{ij}^k C_k = \sum_k \left( \sum_{ij} \alpha_i \alpha_j D_{ij}^k \right) C_k$$

$$= \sum_k \left( \sum_i \alpha_i (\lambda_i \alpha_k) \right) C_k = \underbrace{\sum_i \lambda_i \alpha_i}_a \underbrace{\sum_k \alpha_k C_k}_{\vec{\phi}} \propto \vec{\phi}$$

$$\vec{\phi} = \frac{1}{a} \vec{\phi}^2, \text{ then } \vec{\phi}^2 = \vec{\phi} \text{ idempotent.}$$

We will look at these eigenvectors more closely.

### 8.13.3 Construction of character tables (cont.)

We know that  $C_i$ 's are intertwiners, which means when restricted to a specific irrep:

$$\underline{C_i^\mu = \lambda_i^\mu \cdot 1_{V^\mu}} \quad (\text{Schur's lemma})$$

Taking trace/character.

$$\text{LHS} = \text{Tr}_{V^\mu} \sum_{j \in C_i} g_j = m_i \chi^\mu([C_i])$$

$$\text{RHS} = \lambda_i^\mu \cdot n_\mu$$

$$\Rightarrow \boxed{\lambda_i^\mu = \frac{m_i}{n_\mu} \chi^\mu([C_i])}$$

These are actually the eigen values. Why?

$$C_j C_i = \sum_k [D(j)]_{ki} C_k$$

then taking the characters on  $V^\mu$

~~wrong in class.~~

~~$$\chi_\mu(C_j) \chi_\mu(C_i) = \sum_k [D(j)]_{ki} \chi_\mu(C_k)$$~~

~~$$= \lambda_i^\mu \chi_\mu(C_j)$$~~

~~$$\text{i.e.} \quad \sum_k [D(j)]_{ki} \chi_\mu(C_k) = \lambda_j^\mu \chi_\mu(C_i)$$~~

~~$$\text{take } \vec{\chi}_\mu = \begin{pmatrix} \chi_\mu(C_1) \\ \chi_\mu(C_2) \\ \vdots \\ \chi_\mu(C_r) \end{pmatrix} \text{ then}$$~~

~~$$D(j) \vec{\chi}_\mu = \lambda_j \vec{\chi}_\mu \text{ in matrix form.}$$~~

$$\text{Tr}_\mu(C_i C_j) = \text{Tr}_\mu(C_i \cdot \lambda_j^\mu 1_{V^\mu})$$

$$= \lambda_j^\mu \text{Tr}_\mu(C_i)$$

$$= \lambda_j^\mu m_i \chi_\mu([C_i])$$

$$\sum_k \text{Tr}_\mu([D(j)]_{kj} C_k) = \sum_k [D(j)]_{kj} m_k \chi_\mu([C_k])$$

$$\Rightarrow \sum_k [D(j)]_{kj} \vec{\chi}_\mu = \lambda_j^\mu \vec{\chi}_\mu$$

$$\vec{\chi}_\mu = \begin{pmatrix} m_1 \chi_\mu([C_1]) \\ m_2 \chi_\mu([C_2]) \\ \vdots \\ m_r \chi_\mu([C_r]) \end{pmatrix}$$

remaining two unknowns:  $n_\mu, \chi_\mu$

$$\frac{1}{|G|} \sum_i m_i \chi_\mu(C_i) \overline{\chi_\nu(C_i)} = \delta_{\mu\nu}$$

$$\Rightarrow \frac{1}{|G|} \sum_i m_i \lambda_i^\mu \overline{\lambda_i^\nu} = \delta_{\mu\nu} \left( \frac{m_i}{n_\mu} \right)^2 \quad (\equiv \langle \lambda_i^\nu, \lambda_i^\mu \rangle)$$

$$\Rightarrow \begin{cases} n_\mu = \frac{m_i}{\sqrt{\langle \lambda_i^\mu, \lambda_i^\mu \rangle}} \\ \chi_\mu = \frac{\lambda_i^\mu}{\sqrt{\langle \lambda_i^\mu, \lambda_i^\mu \rangle}} \end{cases}$$

Now, back to the assumption about no degeneracy  
once diagonalized all class operators:

$$\lambda_i^\mu = \frac{m_i}{n_\mu} \chi^\mu([C_i])$$

$$\vec{\lambda}^\mu = \{ \lambda_1^\mu, \lambda_2^\mu, \dots, \lambda_r^\mu \}, \quad \vec{\lambda}^\nu = \{ \lambda_1^\nu, \lambda_2^\nu, \dots, \lambda_r^\nu \}$$

$$\text{if } \forall j, \lambda_j^\mu = \lambda_j^\nu, \text{ then}$$

$$\frac{m_j}{n_\mu} \chi^\mu([C_j]) = \frac{m_j}{n_\nu} \chi^\nu([C_j])$$

$\Rightarrow$  which means two characters are proportional to each other  
cannot be because they should be orthogonal!

Diagonalizing all class operators  $\Rightarrow$  full knowledge of  $\underline{n_\mu, \chi_\mu}$

see 陈金全 for examples of finding / using a minimal  
CS Co-I (subset of class operators).

We will just diagonalize all operators.

$$c_i^{(r)} = \frac{m_i}{n_\mu} \chi_\mu([C_i]) \cdot \mathbb{1}_{i=r} \quad \rightarrow \quad \frac{m_i}{n_\mu} \chi_\mu([C_i]) \frac{m_j}{n_\mu} \chi_\mu([C_j]) = \sum_{k=1}^r c_{ij}^k \frac{m_k}{n_\mu} \chi_\mu([C_k])$$

$$\underline{m_i \chi_\mu([C_i]) m_j \chi_\mu([C_j]) = n_\mu \sum_{k=1}^r c_{ij}^k m_k \chi_\mu([C_k])}$$

Now introduce a set of auxiliary variables  $\{y^i, i=1, \dots, r\}$   
 (so we can differentiate between different  $C_i$ 's:  $C_i \rightarrow C_i y^i$ )

$$\Sigma \text{LHS: } \sum_{i=1}^r m_i m_j \chi_\mu([C_i]) \chi_\mu([C_j]) y^i = \sum_{i=1}^r (\psi_i y^i) \psi_j \quad (\psi_i = m_i \chi_\mu([C_i]))$$

$$\Sigma \text{RHS: } \sum_{i=1}^r n_\mu \sum_{k=1}^r c_{ij}^k m_k \chi_\mu([C_k]) y^i = n_\mu \sum_{k=1}^r L_j^k \psi_k$$

$$\text{Define } \lambda = \frac{1}{n_\mu} \sum_{i=1}^r \psi_i y^i \quad (L_j^k = \sum_i c_{ij}^k y^i)$$

$$\Rightarrow \sum_{k=1}^r L_j^k \psi_k = \lambda \psi_j$$

Solving the eigen problem  $(L - \lambda \mathbb{1}) \psi = 0$

and obtain a set of eigenvalues  $\{\lambda_\mu\}$

$$(*) \quad \underline{\lambda_\mu = \frac{1}{n_\mu} \sum_{i=1}^r \overbrace{m_i \chi_\mu([C_i])}^{\psi_i} y^i} \quad \mu=1, \dots, r$$

Note if we set  $y^j = \delta_{ij}$ , we recover our earlier  $\lambda_i^\mu$ .

Now recall the orthogonality relation:

$$\frac{1}{|G|} \sum_i m_i \chi_\mu(C_i) \overline{\chi_\nu(C_i)} = \delta_{\mu\nu} \quad (\text{ortho. of rows})$$

$$\stackrel{\mu=\nu}{\Rightarrow} \sum_{i=1}^r m_i |\chi_\mu(C_i)|^2 = |G|$$

$$|G| = |\chi_\mu([C_i])|^2 \sum_{i=1}^r m_i \left| \frac{\chi_\mu([C_i])}{\chi_\mu([C_i])} \right|^2$$

$$= n_\mu^2 \sum_{i=1}^r m_i \left| \frac{\chi_\mu([C_i])}{n_\mu} \right|^2$$

$$\Rightarrow n_\mu = \left[ \frac{|G|}{\sum_{i=1}^r m_i \left| \frac{\chi_\mu([C_i])}{n_\mu} \right|^2} \right]^{\frac{1}{2}}$$

known from above (\*)

Implementation in practice:

$$S_3 : E ; (12), (13), (23) ; (123), (132)$$

① class operators:  $C_1 = E$

$$C_2 = (12) + (13) + (23) \quad (12)(13) = (132)$$

$$C_3 = (123) + (132) \quad (12)(123) = (1)(23)$$

② class multiplication table:

	$C_1$	$C_2$	$C_3$	
$C_1$	$C_1$	$C_2$	$C_3$	① explain underlined.
$C_2$	$C_2$	$\underline{3C_1 + 3C_3}$	$\underline{2C_2}$	② symmetric
$C_3$	$C_3$	$\underline{2C_2}$	$\underline{2C_1 + C_3}$	( $\because$ abelian)

③  $L_j^k = \sum_i C_{ij}^k y^i$   $3 \times 3$  matrix

$$L_1^1 = C_{11}^1 y^1 + C_{21}^1 y^2 + C_{31}^1 y^3 = y^1 + 0 + 0$$

$$L_1^2 = \sum_i C_{i1}^2 y^i = y^2$$

$$L_1^3 = y^3$$

$$L_2^1 = \sum_i C_{i2}^1 y^i = 3y^2$$

$$L_2^2 = \sum_i C_{i2}^2 y^i \quad L_2^3 = \sum_i C_{i2}^3 y^i$$

$$L_3^1 = \sum_i C_{i3}^1 y^i \quad L_3^2 = \sum_i C_{i3}^2 y^i$$

$$L_3^3 = \sum_i C_{i3}^3 y^i$$

	$C_1$	$C_2$	$C_3$
$C_1$	$C_1$	$C_2$	$C_3$
$C_2$	$C_2$	$3C_1 + 3C_3$	$2C_2$
$C_3$	$C_3$	$2C_2$	$2C_1 + C_3$

$$\hat{L} = \begin{pmatrix} y^1 & y^2 & y^3 \\ 3y^2 & y^1 + 2y^3 & 3y^2 \\ 2y^3 & 2y^2 & y^1 + y^3 \end{pmatrix} = \begin{pmatrix} 1 & 0 & 0 \\ 0 & 1 & 0 \\ 0 & 0 & 1 \end{pmatrix} y^1 + \begin{pmatrix} 0 & 1 & 0 \\ 3 & 0 & 3 \\ 0 & 2 & 0 \end{pmatrix} y^2 + \begin{pmatrix} 0 & 0 & 1 \\ 0 & 2 & 0 \\ 2 & 0 & 1 \end{pmatrix} y^3$$

$$\begin{cases} \lambda_a = y^1 + 3y^2 + 2y^3 \\ \lambda_b = y^1 - 3y^2 + 2y^3 \\ \lambda_c = y^1 + 0y^2 - y^3 \end{cases}$$

$$\lambda_\mu = \sum_{i=1}^r \frac{m_i \chi_\mu([C_i])}{n_\mu} y^i$$

$$n_\mu = \left[ \frac{|G|}{\sum_{i=1}^r m_i \left| \frac{\chi_\mu([C_i])}{n_\mu} \right|^2} \right]^{\frac{1}{2}}$$

write in cols.



④  $\chi_a = n_a (1, 1, 1)$

$$n_a = 1$$

$$\chi_b = n_b (1, -1, 1)$$

$$n_b = 1$$

$$\chi_c = n_c (1, 0, -\frac{1}{2})$$

$$n_c = \left[ \frac{6}{1 + 3 \cdot 0 + 2 \cdot \frac{1}{4}} \right]^{\frac{1}{2}} = 2$$

⑤ Character table

	$[1]$	$3[(12)]$	$2[(123)]$
$1^+$	1	1	1
$1^-$	1	-1	1
2	2	0	-1

Note that in the solution:

$$\begin{cases} \lambda_a = y^1 + 3y^2 + 2y^3 \\ \lambda_b = y^1 - 3y^2 + 2y^3 \\ \lambda_c = y^1 + 0y^2 - y^3 \end{cases}$$

The eigenvalues of  $\hat{C}_2$  is non-degenerate.

This defines a set of unique eigenvectors that diagonalizes all  $\hat{C}_i$ . Which means  $\hat{C}_2$  is a CSCO by itself.

$$\chi_{\mu_1} = n_{\mu_1} \left( \overset{C_1}{\frac{1}{2}}, \overset{C_2}{\frac{3}{3}}, \overset{C_3}{\frac{2}{2}} \right) = (1, 1, 1) \quad (1) \quad (12) \quad (123)$$

$$\chi_{\mu_2} = n_{\mu_2} \left( \frac{1}{1}, \frac{-3}{3}, \frac{2}{2} \right) = (1, -1, 1)$$

$$\chi_{\mu_3} = n_{\mu_3} \left( \frac{1}{1}, \frac{0}{3}, -\frac{1}{2} \right) = (2, 0, -1)$$

$$\begin{aligned} n_{\mu_1} &= n_{\mu_2} = 1 \\ n_{\mu_3} &= 2 \end{aligned} \quad \Leftarrow \quad \left\{ \begin{aligned} & \\ & \\ & \end{aligned} \right.$$

$$\chi_i^\mu = n_{\mu} \frac{\lambda_i^\mu}{m_i}$$

$$m_1 = 1 \quad m_2 = 3 \quad m_3 = 2$$

↳ normalization;

$$\langle \chi_{\mu_1}, \chi_{\mu_1} \rangle = \frac{1}{6} n_{\mu_1}^2 \cdot 6 = 1$$

$$\langle \chi_{\mu_2}, \chi_{\mu_2} \rangle = \frac{1}{6} n_{\mu_2}^2 \cdot 6 = 1$$

$$\begin{aligned} \langle \chi_{\mu_3}, \chi_{\mu_3} \rangle &= \frac{1}{6} n_{\mu_3}^2 (1 + 0 + \frac{1}{4} \times 2) \\ &= \frac{1}{4} n_{\mu_3}^2 = 1 \end{aligned}$$



Projectors:  $\hat{C}_i \hat{C}_j = \sum_k [D_i]_{jk} C_k$

$$\hat{C}_i \cdot \phi_\mu = \lambda_i^\mu \phi_\mu$$

$$\phi_\mu = \sum_i \phi_\mu(C_i) C_i \\ \equiv \phi_\mu^i C_i$$

$$\sum_j \phi_\mu^j \hat{C}_i \hat{C}_j = \lambda_i^\mu \sum_k \phi_\mu^k C_k$$

$$\Rightarrow \sum_{j,k} \phi_\mu^j [D_i]_{jk} C_k = \lambda_i^\mu \sum_k \phi_\mu^k C_k$$

$$\Rightarrow \sum_k \left( \sum_j (D_i^T)_{kj} \phi_\mu^j \right) C_k = \sum_k \lambda_i^\mu \phi_\mu^k C_k$$

$$\Rightarrow \sum_j (D_i^T)_{kj} \phi_\mu^j = \lambda_i^\mu \phi_\mu^k$$

$$\sum_j (D_i^T - \lambda_i^\mu \delta_{jk}) \phi_\mu^j = 0$$

$\phi_\mu$  are eigenvectors of  $D_i^T$  with basis  $\{C_1, C_2, C_3\}$

$$D_2^T = \begin{pmatrix} 3 & & \\ 1 & 2 & \\ & 3 & \end{pmatrix}$$

$$\lambda_2^{\mu_1} = 3 \quad \phi_{\mu_1} \propto (1, 1, 1)^T \leftarrow \chi_{\mu_1(i)}$$

$$\lambda_2^{\mu_2} = -3 \quad \phi_{\mu_2} \propto (1, -1, 1)^T$$

$$\lambda_2^{\mu_3} = 0 \quad \phi_{\mu_3} \propto (2, 0, -1)^T$$

$$P_{\mu_1} = \alpha_{\mu_1} (C_1 + C_2 + C_3)$$

$$P_{\mu_1}^2 = \alpha_{\mu_1}^2 (C_1^2 + C_2^2 + C_3^2 + 2C_1C_2 + 2C_1C_3 + 2C_2C_3)$$

$$= \alpha_{\mu_1}^2 \left( \underline{C_1} + \underline{3C_1} + \underline{3C_3} + \underline{2C_1} + \underline{C_3} + \underline{2C_2} + \underline{2C_3} + \underline{4C_2} \right)$$

$$= 6\alpha_{\mu_1}^2 (C_1 + C_2 + C_3) = \alpha_{\mu_1} (C_1 + C_2 + C_3) \equiv P_{\mu_1}$$

$$\alpha_{\mu_1} = \frac{1}{6}$$

	$C_1$	$C_2$	$C_3$
$C_1$	$C_1$	$C_2$	$C_3$
$C_2$	$C_2$	$3C_1 + 3C_3$	$2C_2$
$C_3$	$C_3$	$2C_2$	$2C_1 + C_3$

$$P_{\mu_1} = \frac{1}{6} (C_1 + C_2 + C_3)$$

$$P_{\mu_2} = \frac{1}{6} (C_1 - C_2 + C_3)$$

$$P_{\mu_3} = \frac{1}{3} (2C_1 - C_3)$$

$$P_{\mu_1} P_{\mu_2} \propto C_1^2 + C_3^2 + 2C_1 C_3 - C_2^2 = C_1 + 2C_1 + C_3 + 2C_3 - (3C_1 + 3C_3) = 0$$

$$\begin{aligned} P_{\mu_1} P_{\mu_3} &\propto (C_1 + C_2 + C_3)(2C_1 - C_3) = 2C_1^2 - C_1 C_3 + 2C_1 C_2 - C_2 C_3 \\ &\quad + 2C_1 C_3 - C_3^2 \\ &= 2C_1 - C_3 + 2C_2 - 2C_2 = 0 \\ &\quad + 2C_3 - (2C_1 + C_3) = 0 \end{aligned}$$

$$\hat{C}_2 P_{\mu_1} = \frac{1}{6} (C_1 C_2 + C_2^2 + C_2 C_3)$$

$$= \frac{1}{6} (C_2 + 3C_1 + 3C_3 + 2C_2) = 3 \cdot \frac{1}{6} (C_1 + C_2 + C_3)$$

$$= \frac{m_2}{n_{\mu_1}} \chi_{\mu_1}([C_2]) \cdot P_{\mu_1}$$

$$(12) P_{\mu_1} = (12) \cdot \frac{1}{6} (e + \underline{(12)} + \underline{(23)} + \underline{(13)} + (123) + (132))$$

$$(12) P_{\mu_2} = \frac{1}{6} ((12) + \underline{e} + \underline{(123)} + \underline{(132)} + (23) + (13))$$

$$= \chi_{\mu_1} \cdot P_{\mu_1}$$

$$= (-1) \cdot P_{\mu_2} = \chi_{\mu_2} \cdot P_{\mu_2}$$

$$T(h) P^{\mu} = \sum_{i,k=1}^{n_{\mu}} M_{ki}^{\mu}(h) P_{ki}^{\mu}$$

$$P_{\mu_3} = P_{\mu_3}'' + P_{\mu_3}'''$$

$$P_{ij}^{\mu} P_{kl}^{\mu} = \delta_{jk} P_{il}^{\mu}$$

$$T(h) P_{ij}^{\mu} = \sum_{k=1}^{n_{\mu}} M_{ki}^{\mu}(h) P_{kj}^{\mu}$$

$$\Rightarrow P'' \cdot P''' = 0$$

$$P_{11}^{\mu} P_{21}^{\mu} = 0$$

$$\boxed{S P_{kj}^{\mu}, k=1, \dots, n_{\mu}}$$

$$\text{what if } P'' = e - (13) + (12) - (132) \quad ?$$

$$P''' = e - (12) + (13) - (123)$$

$$\text{satisfy the orthogonality relation } \left\{ \begin{array}{l} P_{\mu_3}'' P_{\mu_3}''' = \delta_{12} P_{\mu_3}'' = 0 \\ P_{\mu_1}'' + P_{\mu_1}''' = P_{\mu_1} \end{array} \right.$$

in principle. find more commuting operators  
to lift degeneracies on the group space  $R_G$   
(  $CSC - II$ ,  $CSC - III$  )

use projectors from subgroups:

$$S_3: \begin{array}{c|c|c} & e & (12) \\ \hline 1 & 1 & 1 \\ -1 & 1 & -1 \end{array}$$

$$\begin{array}{c|c|c} & C_1 & C_2 \\ \hline C_1 & C_1 & C_2 \\ \hline C_2 & C_2 & C_1 \end{array}$$

$$P_{2j}^k: \begin{pmatrix} 0 & 1 \\ 1 & 0 \end{pmatrix}$$

$$\lambda = \pm 1$$

$$P'_1 = \frac{1}{2}(e + (12))$$

$$P'_2 = \frac{1}{2}(e - (12))$$

$$G \supset G_1$$

$$P_{\nu_1}^{\nu} = P^{\nu} P^{\nu_1}$$

$$\begin{aligned} \hookrightarrow P_{\underline{1}}^{\underline{2}} &= P^{\underline{2}} P^{\underline{1}} = \frac{1}{6} (2e - (123) - (132)) (e + \underline{12}) \\ &= \frac{1}{6} (2e + 2(12) - (123) - \underline{+}(13) - (132) \\ &\quad \underline{+} (23)) \end{aligned}$$

$$\begin{cases} P^2 = P'_1 + P'_2 \quad \checkmark \\ P'_1 P'_2 = 0 \end{cases}$$

$$\begin{array}{cc} C_2 + C'_2 & CSC - II \\ \uparrow & \uparrow \\ S_3 & S_2 \end{array}$$

$$(12) P_{\pm}^2 = \pm P_{\pm}^2$$